integer_coding.v
@@ -77,6 +77,7 @@ Arguments deendianize _ _ _ _ : simpl never.
 Arguments rank_eq_dec _ _ _ _ : simpl never.
 Arguments rank_subseteq_dec _ _ _ _ : simpl never.
 
+Notation "'charT'" := (IntType char_signedness char_rank) : int_type_scope.
 Notation "'ucharT'" := (IntType Unsigned char_rank) : int_type_scope.
 Notation "'scharT'" := (IntType Signed char_rank) : int_type_scope.
 Notation "'uintT'" := (IntType Unsigned int_rank) : int_type_scope.
